% generated by Ott 0.25 from: Assoc.ott
\documentclass[11pt]{article}
\usepackage{amsmath,amssymb}
\usepackage{supertabular}
\usepackage{geometry}
\usepackage{ifthen}
\usepackage{alltt}%hack
\geometry{a4paper,dvips,twoside,left=22.5mm,right=22.5mm,top=20mm,bottom=30mm}
\usepackage{color}
\usepackage{mathpartir}

\input{Assoc-ott}

\begin{document}

\section{Examples}
\label{sec:examples}

\[
\mprset{flushleft}
\inferrule* [right=TL] {
  $$\mprset{flushleft}
  \inferrule* [right=Gl] {
    $$\mprset{flushleft}
    \inferrule* [right=Gl] {
      $$\mprset{flushleft}
      \inferrule* [right=Gr] {
        $$\mprset{flushleft}
        \inferrule* [right=Tr] {
          $$\mprset{flushleft}
          \inferrule* [right=Var] {
            \,
          }{[[X |-A X]]}
          \\
          $$\mprset{flushleft}
          \inferrule* [right=Var] {
            \,
          }{[[Y |-A Y]]}
        }{[[X,Y |-A X >= Y]]}
      }{[[X,Y |-L g(X >= Y)]]}
    }{[[h(g X),Y |-L g(X >= Y)]]}
  }{[[h(g X), h(g Y) |-L g(X >= Y)]]}
}{[[h(g X) > h(g Y) |-L g(X >= Y)]]}
\]

\[
\mprset{flushleft}
\inferrule* [right=Gl] {
  $$\mprset{flushleft}
  \inferrule* [right=Tl] {
    $$\mprset{flushleft}
    \inferrule* [right=Tr] {
      $$\mprset{flushleft}
      \inferrule* [right=Gr] {
        $$\mprset{flushleft}
        \inferrule* [right=Var] {
          \,
        }{[[X |-A X]]}
      }{[[X |-L g X]]}
      \\
      $$\mprset{flushleft}
      \inferrule* [right=Gr] {
        $$\mprset{flushleft}
        \inferrule* [right=Var] {
          \,
        }{[[Y |-A Y]]}
      }{[[Y |-L g Y]]}
    }{[[X, Y |-L h(g X) > g Y]]}
  }{[[X >= Y |-L h(g X) > g Y]]}
}{[[g(X >= Y) |-L h(g X) > g Y]]}
\]

Using the above two proofs with cut we can show that:
\[
  \begin{array}{c}
    [[(h(g F A) > h(g F B)) > h(g F C) |-L h(g F A) > (h(g F B) > h(g F C))]]\\
    \text{ if and only if }\\
    [[g((F A >= F B) >= F C) |-L g(F A >= (F B >= F C))]]\\
    \text{ if and only if }\\
    [[(F A >= F B) >= F C |-A F A >= (F B >= F C)]]
  \end{array}
\]
Similarly, we have the following:
\[
  \begin{array}{c}
    [[h(g F A) > (h(g F B) > h(g F C)) |-L (h(g F A) > h(g F B)) > h(g F C)]]\\
    \text{ if and only if }\\
    [[g(F A >= (F B >= F C)) |-L g((F A >= F B) >= F C)]]\\
    \text{ if and only if }\\
    [[F A >= (F B >= F C) |-A (F A >= F B) >= F C]]
  \end{array}
\]  
% section examples (end)

\appendix

\section*{Appendix}
\label{sec:appendix}
\section{Full Specification}
\label{sec:full_specification}
\ottall
% section full_specification (end)
% section appendix (end)


\end{document}
